src/examples/simple_base.v
@@ -26,17 +26,23 @@ Section simple_increment.
     let: "ℓ" := ref #4
     in !"ℓ".
 
-  Lemma wp_load_store TV :
-    {{{ True }}} ThreadState alloc_load TV {{{ TV', RET ThreadVal (#4) TV'; True }}}.
+  Lemma wp_load_store SV PV :
+    {{{ validV SV }}} ThreadState alloc_load (SV, PV, ∅) {{{ TV', RET ThreadVal (#4) TV'; True }}}.
   Proof.
-    iIntros (Φ) "_ Post".
+    iIntros (Φ) "#val Post".
     rewrite /alloc_load.
     wp_alloc ℓ as "pts".
     wp_pures.
-  Abort.
-  (*   iModIntro. *)
-  (*   by iApply "Post". *)
-  (* Qed. *)
+    iApply (wp_load with "[$pts $val]").
+    iNext. iIntros (t v) "[pts [%look gt]]".
+    move: look.
+    rewrite /initial_history.
+    rewrite -lookup_fmap.
+    rewrite map_fmap_singleton.
+    intros [<- <-]%lookup_singleton_Some.
+    iApply "Post".
+    done.
+  Qed.
 
   Definition incr_both (ℓ1 ℓ2 : loc) : expr :=
     #ℓ1 <- #1 ;;
